Increased parallel build levels of core theories (#1126)
* Increased parallel build levels of core theories:

- derivativeTheory no more depends on seqTheory
- integrationTheory no more depends on transcTheory

* FTBFS (examples/dependability) due to theorems moved from util_prob to iterateTheory

* Removed PAIRED_BETA_THM (it's actually UNCURRY)

* Removed NUM_2D_BIJ_npair and NUM_2D_BIJ_nfst_nsnd (use BIJ_PAIR_TO_NUM and BIJ_NUM_TO_PAIR instead)

* Further improvements on core builds parallelisation:

- integrationTheory no more depends on limTheory and seqTheory;
- extrealTheory no more util_probTheory

src/real/analysis/derivativeScript.sml
@@ -23,7 +23,7 @@ open numTheory numLib unwindLib tautLib Arith prim_recTheory pairTheory
 
 open realTheory realLib topologyTheory cardinalTheory;
 
-open hurdUtils iterateTheory seqTheory real_topologyTheory;
+open hurdUtils iterateTheory real_topologyTheory;
 
 val _ = new_theory "derivative";
 
@@ -49,8 +49,9 @@ val LIM                = LIM_DEF;            (* real_topologyTheory *)
 
 val exp_ser = “\n. inv(&(FACT n))”;
 
-val exp = new_definition("exp", (* moved from transcTheory *)
-   “exp(x) = suminf(\n. (^exp_ser) n * (x pow n))”);
+Definition exp_def :
+    exp(x) = infsum UNIV (\n. (^exp_ser) n * (x pow n))
+End
 
 (* ------------------------------------------------------------------------- *)
 (* convex                                                                    *)
@@ -1895,40 +1896,18 @@ Proof
   ASM_SIMP_TAC arith_ss [REAL_ADD_COMM]
 QED
 
-val lemma_sums_eq = prove (
-  ``!l x. (seq$sums (\n. ((\n. inv(&(FACT n)))) n * (x pow n)) l) =
-     ((\n. ((\n. inv(&(FACT n)))) n * (x pow n)) sums l) UNIV``,
-  RW_TAC std_ss [sums_def, sums, LIM_SEQUENTIALLY, SEQ, GE] THEN
-  EQ_TAC THEN RW_TAC std_ss [INTER_UNIV] THEN
-  FIRST_X_ASSUM (MP_TAC o Q.SPEC `e`) THEN
-  ASM_REWRITE_TAC [] THEN STRIP_TAC THENL
-  [Q.EXISTS_TAC `N` THEN RW_TAC std_ss [] THEN
-   FIRST_X_ASSUM (MP_TAC o Q.SPEC `SUC n`) THEN
-   ASM_SIMP_TAC arith_ss [dist] THEN
-   REWRITE_TAC [SIMP_RULE std_ss [] lemma_sum_eq],
-   ALL_TAC] THEN
-  Q.EXISTS_TAC `SUC N` THEN RW_TAC std_ss [] THEN
-  FIRST_X_ASSUM (MP_TAC o Q.SPEC `PRE n`) THEN
-  ASM_SIMP_TAC arith_ss [dist] THEN
-  `?m. PRE n = m` by ASM_SIMP_TAC arith_ss [] THEN
-  `n = SUC m` by ASM_SIMP_TAC arith_ss [] THEN
-  ASM_REWRITE_TAC [SIMP_RULE std_ss [] lemma_sum_eq]);
-
 (* cf. transcTheory.EXP_CONVERGES *)
-val EXP_CONVERGES = store_thm ("EXP_CONVERGES",
- ``!z. ((\n. z pow n / (&(FACT n))) sums exp(z)) (from 0)``,
-  SIMP_TAC std_ss [exp] THEN
-  Q_TAC SUFF_TAC `!z. suminf (\n. inv (&FACT n) * z pow n) =
-                 infsum UNIV (\n. inv (&FACT n) * z pow n)` THENL
-  [DISC_RW_KILL,
-   SIMP_TAC std_ss [suminf, suminf_def] THEN
-   SIMP_TAC std_ss [FROM_0, SIMP_RULE std_ss [] (GSYM lemma_sums_eq)]] THEN
-  ONCE_REWRITE_TAC [REAL_MUL_COMM] THEN REWRITE_TAC [GSYM real_div, FROM_0] THEN
-  GEN_TAC THEN SIMP_TAC std_ss [SUMS_INFSUM, summable_def, SERIES_CAUCHY] THEN
-  REWRITE_TAC[INTER_UNIV] THEN
-  MP_TAC(Q.SPEC `abs(z) + &1` EXP_CONVERGES_UNIFORMLY_CAUCHY) THEN
-  SIMP_TAC std_ss [REAL_ARITH ``&0 <= x ==> &0 < x + &1:real``, ABS_POS] THEN
-  METIS_TAC [REAL_ARITH ``x:real <= x + &1``]);
+Theorem EXP_CONVERGES :
+    !z. ((\n. z pow n / (&(FACT n))) sums exp(z)) (from 0)
+Proof
+    RW_TAC std_ss [exp_def, FROM_0]
+ >> ONCE_REWRITE_TAC [REAL_MUL_COMM] >> REWRITE_TAC [GSYM real_div]
+ >> SIMP_TAC std_ss [SUMS_INFSUM, summable_def, SERIES_CAUCHY]
+ >> REWRITE_TAC[INTER_UNIV]
+ >> MP_TAC(Q.SPEC `abs(z) + &1` EXP_CONVERGES_UNIFORMLY_CAUCHY)
+ >> SIMP_TAC std_ss [REAL_ARITH ``&0 <= x ==> &0 < x + &1:real``, ABS_POS]
+ >> METIS_TAC [REAL_ARITH ``x:real <= x + &1``]
+QED
 
 val EXP_CONVERGES_UNIQUE = store_thm ("EXP_CONVERGES_UNIQUE",
  ``!w z. ((\n. z pow n / (&(FACT n))) sums w) (from 0) <=> (w = exp(z))``,
