src/real/analysis/seqScript.sml
@@ -1726,79 +1726,6 @@ val SUMS_ZERO = store_thm
 
 Theorem LT_SUC'[local] = DECIDE “!a b. a < SUC b = a < b \/ (a = b)”
 
-val K_PARTIAL = store_thm
-  ("K_PARTIAL", ``!x. K x = \z. x``, RW_TAC std_ss [K_DEF]);
-
-val HALF_POS = store_thm
-  ("HALF_POS", ``0:real < 1/2``,
-   PROVE_TAC [REAL_ARITH ``0:real < 1``, REAL_LT_HALF1]);
-
-val HALF_LT_1 = store_thm
-  ("HALF_LT_1", ``1 / 2 < 1:real``,
-   ONCE_REWRITE_TAC [GSYM REAL_INV_1OVER, GSYM REAL_INV1]
-   >> MATCH_MP_TAC REAL_LT_INV
-   >> RW_TAC arith_ss [REAL_LT]);
-
-val HALF_CANCEL = store_thm
-  ("HALF_CANCEL", ``2 * (1 / 2) = 1:real``,
-   Suff `2 * inv 2 = 1:real` >- PROVE_TAC [REAL_INV_1OVER]
-   >> PROVE_TAC [REAL_MUL_RINV, REAL_ARITH ``~(2:real = 0)``]);
-
-val X_HALF_HALF = store_thm
-  ("X_HALF_HALF", ``!x:real. 1/2 * x + 1/2 * x = x``,
-   STRIP_TAC
-   >> MATCH_MP_TAC (REAL_ARITH ``(2 * (a:real) = 2 * b) ==> (a = b)``)
-   >> RW_TAC std_ss [REAL_ADD_LDISTRIB, REAL_MUL_ASSOC, HALF_CANCEL]
-   >> REAL_ARITH_TAC);
-
-val ONE_MINUS_HALF = store_thm
-  ("ONE_MINUS_HALF", ``(1:real) - 1 / 2 = 1 / 2``,
-   MP_TAC (Q.SPEC `1` X_HALF_HALF)
-   >> RW_TAC real_ss []
-   >> MATCH_MP_TAC (REAL_ARITH ``((x:real) + 1 / 2 = y + 1 / 2) ==> (x = y)``)
-   >> RW_TAC std_ss [REAL_SUB_ADD]);
-
-(* from util_probTheory, TODO: move to pred_setTheory *)
-val NUM_2D_BIJ_BIG_SQUARE = store_thm
-  ("NUM_2D_BIJ_BIG_SQUARE",
-   ``!(f : num -> num # num) N.
-       BIJ f UNIV (UNIV CROSS UNIV) ==>
-       ?k. IMAGE f (count N) SUBSET count k CROSS count k``,
-   RW_TAC std_ss [IN_CROSS, IN_COUNT, SUBSET_DEF, IN_IMAGE, IN_COUNT]
-   >> Induct_on `N` >- RW_TAC arith_ss []
-   >> Strip
-   >> Cases_on `f N`
-   >> REWRITE_TAC [prim_recTheory.LESS_THM]
-   >> Q.EXISTS_TAC `SUC (MAX k (MAX q r))`
-   >> Know `!a b. a < SUC b = a <= b`
-   >- (KILL_TAC
-       >> DECIDE_TAC)
-   >> RW_TAC std_ss []
-   >> RW_TAC std_ss []
-   >> PROVE_TAC [X_LE_MAX, LESS_EQ_REFL, LESS_IMP_LESS_OR_EQ]);
-
-(* from util_probTheory, TODO: move to pred_setTheory *)
-val NUM_2D_BIJ_SMALL_SQUARE = store_thm
-  ("NUM_2D_BIJ_SMALL_SQUARE",
-   ``!(f : num -> num # num) k.
-       BIJ f UNIV (UNIV CROSS UNIV) ==>
-       ?N. count k CROSS count k SUBSET IMAGE f (count N)``,
-   Strip
-   >> (MP_TAC o
-       Q.SPECL [`f`, `UNIV CROSS UNIV`, `count k CROSS count k`] o
-       INST_TYPE [``:'a`` |-> ``:num # num``]) BIJ_FINITE_SUBSET
-   >> RW_TAC std_ss [CROSS_SUBSET, SUBSET_UNIV, FINITE_CROSS, FINITE_COUNT]
-   >> Q.EXISTS_TAC `N`
-   >> RW_TAC std_ss [SUBSET_DEF, IN_IMAGE, IN_COUNT]
-   >> Q.PAT_X_ASSUM `BIJ a b c` MP_TAC
-   >> RW_TAC std_ss [BIJ_DEF, SURJ_DEF, IN_UNIV, IN_CROSS]
-   >> POP_ASSUM (MP_TAC o Q.SPEC `x`)
-   >> RW_TAC std_ss []
-   >> Q.EXISTS_TAC `y`
-   >> RW_TAC std_ss []
-   >> Suff `~(N <= y)` >- DECIDE_TAC
-   >> PROVE_TAC []);
-
 val SUMINF_ADD = store_thm
   ("SUMINF_ADD",
    ``!f g.
@@ -2128,8 +2055,7 @@ val SER_POS_COMPARE = store_thm
 Theorem SEQ_REAL_SUM_IMAGE :
     !s. FINITE s ==>
         !f f'. (!x. x IN s ==> (\n. f n x) --> f' x) ==>
-                (\n. REAL_SUM_IMAGE (f n) s) -->
-                REAL_SUM_IMAGE f' s
+                (\n. REAL_SUM_IMAGE (f n) s) --> REAL_SUM_IMAGE f' s
 Proof
    Suff `!s. FINITE s ==>
                 (\s. !f f'. (!x. x IN s ==> (\n. f n x) --> f' x) ==>
@@ -2143,6 +2069,85 @@ Proof
    >> POP_ORW
    >> MATCH_MP_TAC SEQ_ADD
    >> METIS_TAC []
+QED
+
+Theorem POW_HALF_SMALL :
+    !e:real. 0 < e ==> ?n. (1 / 2) pow n < e
+Proof
+    RW_TAC std_ss []
+ >> MP_TAC (Q.SPEC `1 / 2` SEQ_POWER)
+ >> RW_TAC std_ss [abs, HALF_LT_1, HALF_POS, REAL_LT_IMP_LE, SEQ]
+ >> POP_ASSUM (MP_TAC o Q.SPEC `e`)
+ >> RW_TAC std_ss [REAL_SUB_RZERO, POW_HALF_POS, REAL_LT_IMP_LE,
+                   GREATER_EQ]
+ >> PROVE_TAC [LESS_EQ_REFL]
+QED
+
+Theorem POW_HALF_MONO :
+    !m n. m <= n ==> ((1:real)/2) pow n <= (1/2) pow m
+Proof
+    REPEAT STRIP_TAC
+ >> Induct_on `n`
+ >- (STRIP_TAC \\
+     Know `m:num = 0` >- DECIDE_TAC \\
+     PROVE_TAC [REAL_LE_REFL])
+ >> Cases_on `m = SUC n` >- PROVE_TAC [REAL_LE_REFL]
+ >> ONCE_REWRITE_TAC [pow]
+ >> STRIP_TAC
+ >> Know `m:num <= n` >- DECIDE_TAC
+ >> STRIP_TAC
+ >> Suff `(2:real) * ((1/2) * (1/2) pow n) <= 2 * (1/2) pow m`
+ >- PROVE_TAC [REAL_ARITH ``0:real < 2``, REAL_LE_LMUL]
+ >> Suff `((1:real)/2) pow n <= 2 * (1/2) pow m`
+ >- (KILL_TAC \\
+     PROVE_TAC [GSYM REAL_MUL_ASSOC, HALF_CANCEL, REAL_MUL_LID])
+ >> PROVE_TAC [REAL_ARITH ``!x y. 0:real < x /\ x <= y ==> x <= 2 * y``,
+               POW_HALF_POS]
+QED
+
+Theorem HARMONIC_SERIES_POW_2 : (* was in util_probTheory *)
+    summable (\n. inv (&(SUC n) pow 2))
+Proof
+    MATCH_MP_TAC POS_SUMMABLE
+ >> CONJ_TAC >- rw []
+ >> Q.EXISTS_TAC `2`
+ >> GEN_TAC
+ >> Cases_on `n` >- rw [sum]
+ >> rename1 ‘sum (0,SUC m) (\n. inv (&SUC n pow 2)) <= 2’
+ >> MATCH_MP_TAC REAL_LE_TRANS
+ >> Q.EXISTS_TAC `1 + sum (1,m) (\n. inv (&n) - inv (&SUC n))`
+ >> CONJ_TAC
+ >- (Know `sum (0,SUC m) (\n. inv (&SUC n pow 2)) =
+           sum (0,1) (\n. inv (&SUC n pow 2)) + sum (1,m) (\n. inv (&SUC n pow 2))`
+     >- (MATCH_MP_TAC EQ_SYM \\
+         MP_TAC (Q.SPECL [`\n. inv (&SUC n pow 2)`, `1`, `m`] SUM_TWO) \\
+         RW_TAC arith_ss [ADD1]) >> Rewr' \\
+     Know `sum (0,1) (\n. inv (&SUC n pow 2)) = 1`
+     >- (REWRITE_TAC [sum, ONE] >> rw []) >> Rewr' \\
+     REWRITE_TAC [REAL_LE_LADD] \\
+     MATCH_MP_TAC realTheory.SUM_LE \\
+     RW_TAC real_ss [REAL_INV_1OVER] \\
+    `&r <> 0` by RW_TAC real_ss [] \\
+    `&SUC r <> 0` by RW_TAC real_ss [] \\
+     ASM_SIMP_TAC real_ss [REAL_SUB_RAT] \\
+    `&SUC r - &r = 1` by METIS_TAC [REAL, REAL_ADD_SUB] >> POP_ORW \\
+     ASM_SIMP_TAC std_ss [POW_2, GSYM REAL_INV_1OVER] \\
+    `0 < &SUC r * &SUC r` by rw [] \\
+     Know `0 < &(r * SUC r)`
+     >- (rw [] >> `0 = r * 0` by RW_TAC arith_ss [] >> POP_ORW \\
+         rw [LT_MULT_LCANCEL]) >> DISCH_TAC \\
+     MATCH_MP_TAC REAL_LT_IMP_LE \\
+     ASM_SIMP_TAC real_ss [REAL_INV_LT_ANTIMONO] \\
+    `SUC r ** 2 = SUC r * SUC r` by RW_TAC arith_ss [] >> POP_ORW \\
+     RW_TAC arith_ss [LT_MULT_RCANCEL])
+ >> `2 = 1 + (1 :real)` by RW_TAC real_ss [] >> POP_ORW
+ >> REWRITE_TAC [REAL_LE_LADD]
+ >> Q.ABBREV_TAC `f = \n. -inv (&n)`
+ >> Know `!n. inv (&n) - inv (&SUC n) = f (SUC n) - f n`
+ >- (RW_TAC real_ss [Abbr `f`] \\
+     REAL_ASM_ARITH_TAC) >> Rewr'
+ >> REWRITE_TAC [SUM_CANCEL]
+ >> rw [Abbr `f`, REAL_SUB_NEG2, REAL_LE_SUB_RADD, REAL_LE_ADDR]
 QED
 
 val _ = export_theory();
